vale/code/arch/x64/interop/Vale.AsLowStar.Wrapper.fst
@@ -18,10 +18,10 @@ module LSig = Vale.AsLowStar.LowStarSig
 // open Vale.AsLowStar.Signature
 // open Vale.AsLowStar.Util
 // friend X64.Interop_s
-friend X64.Memory
-friend X64.Vale.Decls
-friend X64.Vale.StateLemmas
-friend X64.Memory_Sems
+// friend X64.Memory
+// friend X64.Vale.Decls
+// friend X64.Vale.StateLemmas
+// friend X64.Memory_Sems
 // module B = LowStar.Buffer
 // module BV = LowStar.BufferView
 // module HS = FStar.HyperStack
@@ -34,7 +34,7 @@ friend X64.Memory_Sems
 // module VSig = Vale.AsLowStar.ValeSig
 // module LSig = Vale.AsLowStar.LowStarSig
 // module TS = X64.Taint_Semantics_s
-// module SL = X64.Vale.StateLemmas
+module SL = X64.Vale.StateLemmas
 // module BS = X64.Bytes_Semantics_s
 // module MS = X64.Memory_Sems
 
@@ -56,187 +56,88 @@ let create_initial_vale_state
 let lemma_create_initial_vale_state_core
     (args:IX64.arity_ok arg)
     (h0:HS.mem)
-    (stack:ME.b8{mem_roots_p h0 (IX64.arg_of_b8 stack::args)})
+    (stack:IM.b8{mem_roots_p h0 (IX64.arg_of_b8 stack::args)})
   : Lemma
       (ensures (
         let s = create_initial_vale_state args h0 stack in
-        VS.(ME.(s.mem.hs)) == h0
+        Interop.Adapters.hs_of_mem VS.(s.mem) == h0
       ))
-  = admit()
+  = Interop.Adapters.mk_mem_injective (IX64.arg_of_b8 stack::args) h0
 
-// let core_create_lemma
-//     (acc:list ME.b8)
-//     (regs:IS.registers)
-//     (xmms:IS.xmms_t)
-//     (taint:IS.taint_map)
-//     (h0:HS.mem)
-//     (stack:ME.b8{IS.mem_roots_p h0 (stack::acc)})
-//   : Lemma
-//       (ensures (fst (IS.create_initial_trusted_state_core acc regs xmms taint h0 stack) ==
-//                 SL.state_to_S (create_initial_vale_state_core acc regs xmms taint h0 stack)))
-//   =
-//     let s_init, mem = IS.create_initial_trusted_state_core acc regs xmms taint h0 stack in
-//     let s0 = create_initial_vale_state_core acc regs xmms taint h0 stack in
-//     let s1 = SL.state_to_S s0 in
-//     assert (FunctionalExtensionality.feq (SL.regs' s1.TS.state) (SL.regs' s_init.TS.state));
-//     assert (FunctionalExtensionality.feq (SL.xmms' s1.TS.state) (SL.xmms' s_init.TS.state))
+let core_create_lemma
+    (args:IX64.arity_ok arg)
+    (h0:HS.mem)
+    (stack:b8{mem_roots_p h0 (IX64.arg_of_b8 stack::args)})
+  : Lemma
+      (ensures (fst (IX64.create_initial_trusted_state args h0 stack) ==
+                SL.state_to_S (create_initial_vale_state args h0 stack)))
+  = admit() //needs the definition of SL.state_to_S; not sure why its hidden in StateLemma
+module ST = FStar.HyperStack.ST
 
-// [@IS.reduce]
-// let initial_vale_state_t (dom:list IS.vale_type) (acc:list ME.b8) =
-//   IS.initial_state_t dom acc V.va_state
+let code_equiv : squash (V.va_code == TS.tainted_code) = admit()
 
-// [@IS.reduce]
-// let create_vale_initial_state_t (dom:list IS.vale_type)
-//                                 (acc:list ME.b8)
-//     = IS.n_dep_arrow
-//           dom
-//           (initial_vale_state_t dom acc)
+let rec wrap_aux
+         (code:V.va_code)
+         (dom:list td)
+         (args:list arg{List.length args + List.length dom < IX64.max_arity})
+         (num_stack_slots:nat)
+         (pre:VSig.vale_pre_tl dom)
+         (post:VSig.vale_post_tl dom)
+         (v:VSig.vale_sig_tl args code pre post)
+    : LSig.as_lowstar_sig_tl args num_stack_slots pre post
+    = match dom with
+      | [] ->
+        let code : TS.tainted_code = coerce code in
+        let f : LSig.as_lowstar_sig_tl #[] args num_stack_slots pre post =
+          fun () ->
+            let h0 = ST.get () in
+            let f_predict
+                (s0:TS.traceState)
+                (push_h0:mem_roots args)
+                (alloc_push_h0:mem_roots args)
+                (b:IX64.stack_buffer{mem_roots_p alloc_push_h0 (IX64.arg_of_b8 b::args)})
+              : Ghost (nat & ME.mem)
+                  (requires IX64.prediction_pre code args h0 s0 push_h0 alloc_push_h0 b)
+                  (ensures IX64.prediction_post code args h0 s0 push_h0 alloc_push_h0 b)
+                = admit()
+                // let va_s0 = elim_down_nil acc v_down alloc_push_h0 b in
+                // let va_s1, fuel = elim_vale_sig_nil pre post v va_s0 (to_b8 b) in
+                // (fuel, va_s1.mem)
+            in
+            let predict : IX64.prediction code args h0 = f_predict in
+            let IX64.As_lowstar_sig_ret push_h0 alloc_push_h0 b fuel final_mem =
+              IX64.wrap code args h0 predict
+            in
+            admit()
+            // let h1 = get () in
+            // assert (
+            //   let initial_state = elim_down_nil acc v_down alloc_push_h0 b in
+            //   let (final, fuel) = elim_vale_sig_nil pre post v initial_state b in
+            //   eval_code code initial_state fuel final
+            // );
+            // ()
+        in
+        f <: LSig.as_lowstar_sig_tl #[] args num_stack_slots pre post
+      | hd::tl ->
+        let f (x:td_as_type hd) =
+          wrap_aux
+              code
+              tl
+              ((|hd,x|)::args)
+              num_stack_slots
+              (elim_1 pre x)
+              (elim_1 post x)
+              (VSig.elim_vale_sig_cons hd tl args pre post v x)
+        in
+        f
 
-// [@IS.reduce]
-// let create_vale_initial_state
-//       (dom:sig_arity_ok)
-//     : create_vale_initial_state_t dom []
-//     = IS.create_initial_state_aux
-//           dom
-//           IA.win
-//           0
-//           IA.init_regs
-//           IA.init_xmms
-//           []
-//           IS.init_taint
-//           create_initial_vale_state_core
 
-// [@IS.reduce]
-// let elim_down_nil (acc:list ME.b8)
-//                   (down:create_vale_initial_state_t [] acc)
-//     : h0:HS.mem -> stack:ME.b8{IS.mem_roots_p h0 (stack::acc)} -> GTot V.va_state =
-//     down
-
-// [@IS.reduce]
-// let elim_down_cons (hd:IS.vale_type)
-//                    (tl:list IS.vale_type)
-//                    (acc:list ME.b8)
-//                    (down:create_vale_initial_state_t (hd::tl) acc)
-//                    (x:IS.vale_type_as_type hd)
-//     : create_vale_initial_state_t tl (IS.maybe_cons_buffer hd x acc) =
-//     IS.elim_dep_arrow_cons hd tl down x
-
-// let rec n_dep_arrow_equiv (dom:list IS.vale_type)
-//                           (acc:list ME.b8)
-//                           (f:IS.create_trusted_initial_state_t dom acc)
-//                           (g:create_vale_initial_state_t dom acc) =
-//     match dom with
-//     | [] ->
-//       forall h0 (stack:ME.b8{IS.mem_roots_p h0 (stack::acc)}).
-//         fst (IS.elim_down_nil acc f h0 stack) == SL.state_to_S (elim_down_nil acc g h0 stack)
-
-//     | hd::tl ->
-//       forall (x:IS.vale_type_as_type hd).
-//         n_dep_arrow_equiv tl (IS.maybe_cons_buffer hd x acc)
-//                              (IS.elim_down_cons hd tl acc f x)
-//                              (elim_down_cons hd tl acc g x)
-
-// let rec equiv_create_trusted_and_vale_state
-//           (dom:list IS.vale_type)
-//           (i:nat{i + List.length dom < IS.max_arity IA.win})
-//           (regs:_)
-//           (xmms:_)
-//           (acc:list ME.b8)
-//           (taint:_)
-//     : Lemma (n_dep_arrow_equiv
-//                   dom
-//                   acc
-//                   (IS.create_initial_state_aux
-//                       dom
-//                       IA.win
-//                       i
-//                       regs
-//                       xmms
-//                       acc
-//                       taint
-//                       IS.create_initial_trusted_state_core)
-//                   (IS.create_initial_state_aux
-//                       dom
-//                       IA.win
-//                       i
-//                       regs
-//                       xmms
-//                       acc
-//                       taint
-//                       create_initial_vale_state_core))
-//      = match dom with
-//        | [] ->
-//          FStar.Classical.forall_intro_2 (core_create_lemma acc regs xmms taint)
-//        | hd::tl ->
-//          let aux (x:IS.vale_type_as_type hd)
-//            : Lemma (n_dep_arrow_equiv
-//                       tl
-//                       (IS.maybe_cons_buffer hd x acc)
-//                       (IS.create_initial_state_aux
-//                            tl
-//                            IA.win
-//                            (i + 1)
-//                            (IS.update_regs x IA.win i regs)
-//                            xmms
-//                            (IS.maybe_cons_buffer hd x acc)
-//                            (IS.update_taint_map x taint)
-//                            IS.create_initial_trusted_state_core)
-//                       (IS.create_initial_state_aux
-//                            tl
-//                            IA.win
-//                            (i + 1)
-//                            (IS.update_regs x IA.win i regs)
-//                            xmms
-//                            (IS.maybe_cons_buffer hd x acc)
-//                            (IS.update_taint_map x taint)
-//                            create_initial_vale_state_core))
-//          =
-//            equiv_create_trusted_and_vale_state
-//                 tl
-//                 (i + 1)
-//                 (IS.update_regs x IA.win i regs)
-//                 xmms
-//                 (IS.maybe_cons_buffer hd x acc)
-//                 (IS.update_taint_map x taint)
-//           in
-//           FStar.Classical.forall_intro aux
-
-// let rec wrap_tl
-//          (code:V.va_code)
-//          (dom:list IS.vale_type)
-//          (acc:list ME.b8)
-//          (args:LSig.lowstar_args{List.length args + List.length dom < IS.max_arity IA.win})
-//          (num_stack_slots:nat)
-//          (fp:ME.loc)
-//          (v_down:create_vale_initial_state_t dom acc)
-//          (t_down:IS.create_trusted_initial_state_t dom acc{n_dep_arrow_equiv dom acc t_down v_down})
-//          (pre:VSig.vale_pre_tl dom)
-//          (post:VSig.vale_post_tl dom)
-//          (v:VSig.vale_sig_tl fp code IA.win pre post)
-//          (t_low:IS.as_lowstar_sig_tl code dom acc t_down)
-//     : LSig.as_lowstar_sig_tl args num_stack_slots pre post
-//     = admit()
-
-// let wrap
-//     (code:V.va_code)
-//     (dom:sig_arity_ok)
-//     (num_stack_slots:nat)
-//     (pre:VSig.vale_pre dom)
-//     (post:VSig.vale_post dom)
-//     (v:VSig.vale_sig pre post)
-//   : LSig.as_lowstar_sig code dom num_stack_slots pre post
-//   = let is_wrapper = IS.wrap code dom in
-//     equiv_create_trusted_and_vale_state dom 0 IA.init_regs IA.init_xmms [] IS.init_taint;
-//     wrap_tl
-//       code
-//       dom
-//       []
-//       []
-//       num_stack_slots
-//       ME.loc_none
-//       (create_vale_initial_state dom)
-//       (IS.create_trusted_initial_state IA.win dom)
-//       (pre code IA.win)
-//       (post code IA.win)
-//       (v code IA.win)
-//       is_wrapper
+let wrap
+    (code:V.va_code)
+    (dom:IX64.arity_ok td)
+    (num_stack_slots:nat)
+    (pre:VSig.vale_pre dom)
+    (post:VSig.vale_post dom)
+    (v:VSig.vale_sig pre post)
+  : LSig.as_lowstar_sig code dom num_stack_slots pre post
+  = wrap_aux code dom [] num_stack_slots (pre code) (post code) (v code IA.win)
